documentation, drop Array.repeatM

SSA/Core/Framework/Refinement.lean
@@ -159,55 +159,12 @@ variable {x : A a} {xs : HVector A as} {y : B b} {ys : HVector B bs}
 
 end HVector
 
-
-/-!
-## Normal Forms
-
-In a concrete dialect, we expect to have a kind of waterfall of refinement
-instances. Take, for example, the LLVM dialect:
-* Firstly, there is the `PoisonOr _` type, which has a refinement relation.
-* Then, there is the `LLVM.IntW w` type, which is a (semireducible!) alias for
-  `PoisonOr (BitVec w)`. Because it is not reducible, it has its own refinement
-  instance.
-* Using the latter, there is the `DialectHRefinement` instance for the LLVM
-  dialect.
-* This `DialectHRefinement` instance implies refinement instances for both
-  monadic value `LLVM.m ⟦t⟧` and pure values `⟦t⟧`.
-
-Recall, however, that LLVM is a *pure* dialect (that is, `LLVM.m` is `Id`).
-Suppose we had a `MemLLVM` dialect, which also captures memory side effects,
-then we'd expect the following refinement instances:
-* We still start with `PoisonOr _` and `LLVM.IntW _`, and their refinement.
-* Then, we expect some `EffectM` monad, which will have a refinement instance
-  for `EffectM α`, with `α` being some generic type with a refinement instance.
-* Using both of the above, we then define the `DialectHRefinement` instance,
-  which implies the same refinement instances as before.
-
-Note that in either case, the semantics content is defined at the top of the
-list, with the instances after `DialectHRefinement` simply being ways to express
-this refinement for alternative spellings of the same type.
-
-Thus, although a rewrite like `toMonad_pure_IsRefinedBy_toMonad_pure_iff`
-*in general* seems like a good idea (the rhs is a simpler expression, after all),
-for a concrete dialect this rewrite is actually hiding the semantic content by
-going *down* this list of instances.
-
-Luckily, we have a dedicated simpset intended for concrete rewrites, `simp_denote`.
-Thus, we add set of lemmas to this simpset which rewrite the derived instances
-in terms of the original `DialectHRefinement` instance.
-
-We expect dialect implementors to then add their dialect-specific simplemmas to
-`simp_denote`, to go all the way up the list of instances.
--/
-
+/-! ## Canonicalization -/
 section SimpDenote
 open Lean Meta
 open Simp (SimpM)
 
--- TODO: upstream (or drop)
-def Array.replicateM [Monad m] (size : Nat) (x : m α) : m (Array α) :=
-  replicate size () |>.mapM (fun _ => x)
-
+/-- Implementation of `reduceIsRefinedBy` simproc -/
 partial def reduceIsRefinedByAux (α β inst lhs rhs : Expr) : SimpM (Option Expr) := do
   let ⟨instFn, instArgs⟩ := inst.withApp Prod.mk
   trace[LeanMLIR.Elab] "Refinement instance is an application of: {instFn}"
@@ -268,75 +225,33 @@ where
 
 open Lean Meta in
 /--
-`reduceIsRefinedBy` simplifies `HRefinement` instances that are derived by an `DialectHRefinement`
-instance into an application of `DialectHRefinement.IsRefinedBy`.
+`reduceIsRefinedBy` simplifies certain `HRefinement` instances.
 
-NOTE: this simproc matches on *all* occurences of `HRefinement.IsRefinedBy`, which could potentially
-be expensive. Ideally, we'd include the specific instances we're searching for in the discrtree key.
-Furthermore, we have a tendency to rewrite `toType t` into the underlying type,
-so we do *not* want `toType`, or `Dialect.m` or similar methods to be part of the index.
+We tend to have a lot of types which are def-eq, but not *reducibly* def-eq,
+to others. Yet, we often want to write simp-lemmas just about the underlying
+types and not have to duplicate those.
 
-For example, this could be one of the rewrites that are expressed by this simproc:
-```
-theorem monadic_isRefinedBy_iff (x : d.m ⟦t⟧) (y : d'.m ⟦u⟧) :
-    @HRefinement.IsRefinedBy (no_index _) (no_index _) (instRefinementMonadic) x y
-    ↔ DialectHRefinement.IsRefinedBy x y := by rfl
-```
-However, even if we write these rewrites as simp-lemmas: the instances are *not*
-part of the discrtree key indexing, so the above will *also* match against all
-occurences of `HRefinement.IsRefinedBy`.
+In particular, this holds for the denotation of dialect types (i.e., `⟦t⟧` for
+some `t : Dialect.Ty _`), dialect monads (`Dialect.m _`) or even the identity
+monad `Id`. Thus, it is common to define a `DialectHRefinement` instance in
+terms of `inferInstance(As)` and mark the instance as `@[simp_denote]`.
+
+Note that the instances are not problematic, per se, as instances are *not* part
+of the discrtree matching that `simp` uses [1], however, the *types* that are
+passed to `HRefinement.IsRefinedBy` *are* part of the discrtree (unless
+explictly marked `no_index` by a particular simp-lemma). While unfolding the
+instances, `reduceIsRefinedBy` will also unfold the *types* into the canonical
+spelling for the unfolded type.
+
+Using `LLVM` as an example: the base framework will have goals `?lhs ⊑ ?rhs`
+where `?lhs : LLVM.m ⟦?t⟧` and `?t : LLVM.Ty`. Assuming the `DialectHRefinement`
+instance for `LLVM` is marked `@[simp_denote]`, `reduceIsRefinedBy` will
+canonicalize this into a goal `?lhs' ⊑ ?rhs'`, where `?lhs', ?rhs' : LLVM.IntW _`.
 -/
 dsimproc [simp_denote] reduceIsRefinedBy (_ ⊑ _) := fun e => do
   return match ← reduceIsRefinedByAux.loop (returnArgOnFail := false) e with
   | some e => .visit e
   | none => .continue
-
-  -- /-
-  --   TODO: we probably only want to simplify these instances if the dialects `d`
-  --   and `d'` are concrete. Meaning if `d` and `d'` are not just fvars (although
-  --   we probably should allow them to be *contain* fvars, so that, say,
-  --   `MetaLLVM φ` is still considered concrete).
-  -- -/
-
-  -- match_expr inst with
-  -- | instRefinementMonadic d d' tyDenote tyDenote' instRefinement t u =>
-  --     let expr := mkAppN (mkConst ``DialectHRefinement.IsRefinedBy)
-  --       #[d, d', tyDenote, tyDenote', instRefinement, t, u, a, b]
-  --     return .visit expr
-  -- | instRefinementPure d d' tyDenote tyDenote' instRefinement t u instPure instPure' =>
-  --     let a :=
-  --       let Ty := mkApp (mkConst ``Dialect.Ty) d
-  --       let m := mkApp (mkConst ``Dialect.m) d
-  --       let α := mkApp3 (mkConst ``TyDenote.toType) Ty tyDenote t
-  --       mkApp4 (.const ``pure [0, 0]) m instPure α a
-  --     let b :=
-  --       let Ty := mkApp (mkConst ``Dialect.Ty) d'
-  --       let m := mkApp (mkConst ``Dialect.m) d'
-  --       let β := mkApp3 (mkConst ``TyDenote.toType) Ty tyDenote u
-  --       mkApp4 (.const ``pure [0, 0]) m instPure' β b
-  --     let expr := mkAppN (mkConst ``DialectHRefinement.IsRefinedBy)
-  --       #[d, d', tyDenote, tyDenote', instRefinement, t, u, a, b]
-  --     return .visit expr
-  -- | instRefinementEffect d d' tyDenote tyDenote' instRefinement t u instPure instPure' eff eff' =>
-  --     let a :=
-  --       let Ty := mkApp (mkConst ``Dialect.Ty) d
-  --       let m := mkApp (mkConst ``Dialect.m) d
-  --       let α := mkApp3 (mkConst ``TyDenote.toType) Ty tyDenote t
-  --       mkApp5 (mkConst ``EffectKind.coe_toMonad) m α instPure eff a
-  --     let b :=
-  --       let Ty := mkApp (mkConst ``Dialect.Ty) d'
-  --       let m := mkApp (mkConst ``Dialect.m) d'
-  --       let α := mkApp3 (mkConst ``TyDenote.toType) Ty tyDenote' u
-  --       mkApp5 (mkConst ``EffectKind.coe_toMonad) m α instPure' eff' b
-  --     let expr := mkAppN (mkConst ``DialectHRefinement.IsRefinedBy)
-  --       #[d, d', tyDenote, tyDenote', instRefinement, t, u, a, b]
-  --     return .visit expr
-  -- | instHRefinementOfRefinement α instRefinement =>
-  --     match_expr instRefinement with
-  --     | Refinement.ofEq _α =>
-  --         return .visit <| mkApp3 (.const ``Eq [1]) α a b
-  --     | _ => return .continue
-  -- | _ => return .continue
 
 end SimpDenote
 
